% Created 2017-05-06 Sat 08:47
% Intended LaTeX compiler: pdflatex
\documentclass[11pt]{article}
\usepackage[utf8]{inputenc}
\usepackage[T1]{fontenc}
\usepackage{graphicx}
\usepackage{grffile}
\usepackage{longtable}
\usepackage{wrapfig}
\usepackage{rotating}
\usepackage[normalem]{ulem}
\usepackage{amsmath}
\usepackage{textcomp}
\usepackage{amssymb}
\usepackage{capt-of}
\usepackage{hyperref}
\author{Kadin Buckton}
\date{\today}
\title{Solving Rational Equations}
\hypersetup{
 pdfauthor={Kadin Buckton},
 pdftitle={Solving Rational Equations},
 pdfkeywords={},
 pdfsubject={},
 pdfcreator={Emacs 25.2.1 (Org mode 9.0.5)}, 
 pdflang={English}}
\begin{document}

\maketitle
Reminders in solving equations\ldots{}

We isolate the variable through the order of operations (BEDMAS)

\begin{enumerate}
\item Remove fractions by multiplying every term by the common denominator
\item Expand brackets
\item Collect like terms
\item Combine like terms
\end{enumerate}


\section*{Examples}
\label{sec:orgcc12865}

Solve for x.
\begin{align*}
\frac{x+3}{x-4} &= \frac{x-1}{x+2}\\
(x+3)(x+2) &= (x-1)(x-4)\\
x^2+5x+6 &= x^2-5x+4\\
10x &= -2\\
x &= \frac{-1}{5}
\end{align*}

\begin{align*}
\frac{x-3}{x-2} &= 0\\
(x-3) &= 0\\
x &= 3
\end{align*}

\begin{align*}
\frac{3x-1}{x} &= \frac{5}{2}\\
2(3x-1) &= 5x\\
6x-2 &= 5x\\
6x-5x &= 2\\
x &= 2
\end{align*}

\begin{align*}
\frac{2}{x+1}+\frac{1}{x+1} &= 3\\
(x+1)(\frac{2}{x+1}+\frac{1}{x+1}) &= 3\\
2 + 1 &= 3(x+1)\\
1 = x + 1\\
x = 0
\end{align*}
\end{document}